Endpoint for universally quantiefied result of threads

theories/program_logic/delayfree.v
@@ -57,16 +57,15 @@ Instance itree_bind {E}: MBind (itree E) := λ R S k,
     | Vis e k => Vis e (λ x, go (k x))
     end.
 
-
 Instance itree_mret {E}: MRet (itree E) :=
  λ _ x, Answer x.
 
 Instance itree_fmap {E}: FMap (itree E) :=
    λ A B f ma, ma ≫= mret ∘ f.
 
-(* Definition delay_st_pipe {ST A B C} 
-    (f: A -> delay_st ST B)
-    (g: B -> delay_st ST C): A -> delay_st ST C := 
+Definition pipe {M} {m: MBind M} {A B C} 
+    (f: A -> M B)
+    (g: B -> M C): A -> M C := 
   λ x,  f x ≫= g.
 
 Definition case_ {A B C}  (f: A -> C) (g: B -> C)
@@ -77,107 +76,17 @@ Definition case_ {A B C}  (f: A -> C) (g: B -> C)
         | inr b => g b
         end .
   
-CoFixpoint iter {ST A B} (f: A -> delay_st ST (A + B)) : A -> delay_st ST B :=
-    delay_st_pipe f (case_ (Think ∘ iter f) Answer). *)
+CoFixpoint iter {V A B} (f: A -> expr V (A + B)) : A -> expr V B :=
+    pipe f (case_ (Think ∘ iter f) Answer). 
 
-
-Definition heap V := gmap nat V.
-
-Variant step_result (V A: Type): Type :=
-| Step (e: expr V A)
-| ForkStep (e: expr V A) (ef: expr V ()).
-
-Arguments Step {_ _}.
-Arguments ForkStep {_ _}.
-
-Definition step_vis {V R T}
- (c: envE V T)
- : (T -> expr V R) -> state (heap V) (step_result V R) :=
-    match c with
-    |GetE l   => λ k, (Step ∘ k) <$> (state.get l)
-    |PutE l v => λ k, (Step ∘ k) <$> (state.put l v)
-    |AllocE v => λ k, (Step ∘ k) <$> (state.alloc v)
-    |FreeE l  => λ k, (Step ∘ k) <$> (state.free l)
-    end.
-
-Definition step_expr {V R} (e: expr V R): state (heap V) (step_result V R) :=
-    match e with
-    | Answer x  => mret $ Step $ Answer x 
-    | Vis stateE k => step_vis stateE k 
-    | Fork e' k => mret $ ForkStep k e'
-    | Think e'  =>  mret $ Step e'
-    end.
-
-
-Definition step_delay_st_heap {A} (e: delay_st heap A)
-    : state heap (delay_st heap A).
-refine (
-    match e with
-    | Answer x   => mret $ Answer x
-    | Get n k    => _
-    | Put n s' k => _
-    | Think e'   => _
-    end
-).
-- refine(_).
-Admitted.
-
-(* First a single threaded evaluator *)
-Fixpoint eval_delay_st {ST A} (n: nat) (e: delay_st ST A) (s: ST) {struct n} : option A :=
-    match n with
-    | O => None
-    | S n' => match (runState (step_delay_st e) s) with 
-              | Some (e', s') => eval_delay_st n' e' s'
-              | None => None
-              end
-    end.
-
-Fixpoint split_and_circulate {A} (xs: list A) (f: A -> A) {struct xs}: (list A) :=
-    match xs with
-    | nil => nil
-    | cons x xs' => xs' ++ [f x]
-    end.
-
-Definition step_delay_st_threads {ST A} 
-    (threads: list (delay_st ST A)) (s: ST)
-    :(ST * (list (delay_st ST A))) :=
-        match threads with 
-        | nil => (s, nil)
-        | cons e es' => match (runState (step_delay_st e) s) with
-                        | None => (s, nil)
-                        | Some (e', s') => (s', es' ++ [e'])
-                        end
-        end.
-
-Definition check_delay_st {ST A} (e: delay_st ST A): A + delay_st ST A :=
-    match e with
-    | Answer x  => inl x
-    | Get n k     => inr $ e
-    | Put n s' k  => inr $ e
-    | Think e'  => inr $ e
-    end.
-
-(* Todo check the order of effects with list and state here
-   and remove all these nested pattern matches
-*)
-Fixpoint eval_threaded_delay_st {ST A} 
-    (n: nat) 
-    (threads: list (delay_st ST A))
-    (s: ST) {struct n}: option A :=
-
-    match n with
-    | O => None
-    | S n' => let (s', threads') := (step_delay_st_threads threads s)
-              in match threads' with
-                 | nil => None
-                 | cons e' _ => match check_delay_st e' with
-                                | inl x => Some x
-                                | inr e'' => eval_threaded_delay_st n' threads' s'
-                                end
+CoFixpoint loop {V A B C} (f: (C + A) -> expr V (C + B)): A -> expr V B :=
+    λ a, iter (λ ca,
+                 cb ← f ca ;
+                 match cb with
+                 | inl c => mret (inl (inl c))
+                 | inr b => mret (inr b)
                  end
-    end.
-
-
+    ) (inr a).
 
 
 
