theories/program_logic/evaluation.v
@@ -1,0 +1,179 @@
+From stdpp Require Import base gmap list.
+From shiris.program_logic Require Import delayfree.
+
+(* Ask casper how to credit his blog post*)
+
+Definition heap V := gmap nat V.
+
+(* How am I going to differentiate between the main thread that returns a value,
+   And the spawned threads that do not. 
+ *)
+Variant thread (V A: Type): Type :=
+| Main (e: expr V A)
+| Forked (e: expr V ()).
+
+Arguments Main {_ _}.
+Arguments Forked {_ _}.
+
+Instance fmap_thread {V}: FMap (thread V) :=
+  λ A B f fa, match fa with
+              | Main e' => Main $ f <$> e'
+              | Forked e => Forked e
+  end.
+
+
+Record state (V A B: Type): Type := State {
+                                      runState: heap V -> list (thread V A) -> option (B * heap V * list (thread V A))
+                                     }.
+
+Arguments State {_ _ _} .
+Arguments runState {_ _ _} .
+
+Instance fmap_state {V A}: FMap (state V A) :=
+  λ A B f fa, 
+         State $ λ h threads, 
+                  match (runState fa) h threads with
+                  | Some (x, heap, threads) => Some (f x, heap , threads)
+                  | None => None
+                  end.
+
+Instance mret_state {V A} : MRet (state V A) := λ A a, State $ λ h threads, Some (a, h, threads).
+
+Instance mbind_state {V A}: MBind (state V A) :=
+  λ _ _ f ma, State $
+                    λ h threads, match (runState ma) h threads with
+                          | Some (x, h', threads) => runState (f x) h' threads
+                          | None => None
+                          end.
+
+
+Definition modifyS' {V A B} (f: heap V -> B * heap V): state V A B :=
+  State $ λ h t, Some $ (f h, t).
+
+Section state_op.
+   Context {V A B: Type}.
+
+   Definition getS: state V A (heap V) :=
+     State $ λ h t, Some (h, h, t).
+  
+   Definition putS (x: heap V): state V A unit :=
+     State $ λ h t, Some (tt, x, t).
+
+   Definition modifyS (f: heap V -> heap V): state V A () :=
+     modifyS' $ λ h, (tt, f h).
+
+   Definition fail: state V A B :=
+     State $ λ h t, None.
+
+   Definition ret_fail (m: option B): state V A B := 
+    match m with
+    | Some x => mret x
+    | None => fail
+    end.
+
+    Definition fork (e: state V A B) (t: thread V A): state V A B :=
+      State $ λ h ts, (runState e) h (t :: ts).
+    
+    Definition get_thread (n: nat): state V A (thread V A) :=
+      State $ λ h ts, (λ t,( t, h, ts)) <$> ( ts !! n).
+End state_op.
+
+
+Section heap_op.
+  Context {V A B: Type}.
+
+  Definition get (n: nat): state V A V :=
+    getS ≫= λ h, ret_fail $ lookup n h.
+
+  Definition put (n: nat) (x : V) : state V A unit :=
+    modifyS <[n := x]>.
+
+  Definition alloc (v: V) : state V A nat :=
+    modifyS'$ λ st, 
+                let fresh := fresh $ dom (gset nat) st
+                in (fresh, <[fresh := v]> st).
+
+  Definition free (n: nat): state V A unit :=
+    modifyS $ delete n.
+End heap_op.
+
+
+Definition step_vis {V R T}
+ (c: envE V T)
+ : (T -> expr V R) -> state V R (expr V R) :=
+    match c with
+    |GetE l   => λ k, k <$> (get l)
+    |PutE l v => λ k, k <$> (put l v)
+    |AllocE v => λ k, k <$> (alloc v)
+    |FreeE l  => λ k, k <$> (free l)
+    end.
+
+Definition step_expr {V R} (e: expr V R): state V R (expr V R) :=
+    match e with
+    | Answer x  => mret $ Answer x 
+    | Vis stateE k => step_vis stateE k 
+    | Fork e' k => fork (mret k) (Forked e')
+    | Think e'  =>  mret e'
+    end.
+
+
+Fixpoint eval_single {V R} (n: nat) (e: expr V R) {struct n}: state V R (option R) :=
+  match n with
+  | O => mret $ None
+  | S n' => (step_expr e) ≫= (eval_single n') 
+  end. 
+
+Definition step_thread {V A} (t: thread V A) : state V A (thread V A).
+  refine(match t with 
+    | Main e => Main <$> (step_expr e)
+    | Forked e => Forked <$> (step_expr e) 
+    end).
+
+
+Fixpoint split_and_circulate {A} (xs: list A) (f: A -> A) {struct xs}: (list A) :=
+    match xs with
+    | nil => nil
+    | cons x xs' => xs' ++ [f x]
+    end.
+
+Definition step_delay_st_threads {V A} 
+    (threads: list (Thread V A)) (s: heap V)
+    :(heap V * (list (Thread V A))) :=
+        match threads with 
+        | nil => (s, nil)
+        | cons e es' => match (runState (step_expr e) s) with
+                        | None => (s, nil)
+                        | Some (e', s') => (s', es' ++ [e'])
+                        end
+        end.
+
+Definition check_delay_st {ST A} (e: delay_st ST A): A + delay_st ST A :=
+    match e with
+    | Answer x  => inl x
+    | Get n k     => inr $ e
+    | Put n s' k  => inr $ e
+    | Think e'  => inr $ e
+    end.
+
+(* Todo check the order of effects with list and state here
+   and remove all these nested pattern matches
+*)
+Fixpoint eval_threaded_delay_st {ST A} 
+    (n: nat) 
+    (threads: list (delay_st ST A))
+    (s: ST) {struct n}: option A :=
+
+    match n with
+    | O => None
+    | S n' => let (s', threads') := (step_delay_st_threads threads s)
+              in match threads' with
+                 | nil => None
+                 | cons e' _ => match check_delay_st e' with
+                                | inl x => Some x
+                                | inr e'' => eval_threaded_delay_st n' threads' s'
+                                end
+                 end
+    end.
+
+
+
